\documentclass{../../style}
\usepackage{breqn}
\usepackage{amssymb}

\begin{document}
	\begin{center}
		\texttt{Pure Book 1, Exercise 7A}

		\section*{Question 1}
		\begin{subequations}
			\begin{dmath}
				\frac{4x^4 + 5x^2 - 7x}{x} = \frac{x(4x^3 + 5x - 7)}{x} = 4x^3 + 5x - 7
			\end{dmath}
	
			\begin{dmath}
				\frac{7x^5 - 5x^5 + 9x^3 + x^2}{x} = \frac{x(2x^4 + 9x^2 + x)}{x} = 2x^4 + 9x^2 + x
			\end{dmath}
	
			\begin{dmath}
				\frac{-x^4 + 4x^2 + 6}{x} = \frac{x(4x - x^3) + 6}{x} = \frac{x(4x - x^3)}{x} + \frac{6}{x} = 4x - x^3 + \frac{6}{x}
			\end{dmath}

			\begin{dmath}
				\frac{7x^5 - x^3 - 4}{x} = \frac{x(7x^4 - x^2) - 4}{x} = \frac{x(7x^4 - x^2)}{x} - \frac{4}{x} = 7x^4 - x^2 - \frac{4}{x}
			\end{dmath}

			\begin{dmath}
				\frac{8x^4 - 4x^3 + 6x}{2x} = \frac{2x(4x^3 - 2x^2 + 3)}{2x} = 4x^3 - 2x^2 + 3
			\end{dmath}

			\begin{dmath}
				\frac{9x^2 - 12x^3 - 3x}{3x} = \frac{3x(3x - 4x^2 - 1)}{3x} = -4x^2 + 3x - 1
			\end{dmath}

			\begin{dmath}
				\frac{7x^3 - x^4 - 2}{5x} = \frac{x(7x^2 - x^3)}{x(5)} - \frac{2}{5x} = -\frac{1}{5}x^3 + \frac{7}{5}x^2 - \frac{2}{5x}
			\end{dmath}

			\begin{dmath}
				\frac{-4x^2 + 6x^4 - 2x}{-2x} = \frac{-2x(2x - 3x^3 + 1)}{-2x} = -3x^3 + 2x + 1
			\end{dmath}

			\begin{dmath}
				\frac{-x^8 + 9x^4 - 4x^3 + 6}{-2x} = \frac{-x(x^7 - 9x^3 + 4x^2)}{-x(2)} + \frac{-2(-3)}{-2x} = \frac{1}{2}x^7 - \frac{9}{2}x^3 + 2x^2 - \frac{3}{x}
			\end{dmath}

			\begin{dmath}
				\frac{-9x^9 - 6x^6 + 4x^4 - 2}{-3x} = \frac{-x(9x^8 + 6x^5 - 4x^3)}{-x(3)} - \frac{2}{-3x} = 3x^8 + 2x^5 - \frac{4}{3}x^3 + \frac{2}{3x}
			\end{dmath}
		\end{subequations}

		\section*{Question 2}
		\begin{subequations}
			\begin{dmath}
				\frac{(x + 3)(x - 2)}{(x - 2)} = x + 3
			\end{dmath}

			\begin{dmath}
				\frac{(x + 4)(3x - 1)}{(3x - 1)} = x + 4
			\end{dmath}

			\begin{dmath}
				\frac{(x + 3)^2}{(x + 3)} = x + 3
			\end{dmath}

			\begin{dmath}
				\frac{x^2 + 10x + 21}{(x + 3)} = \frac{(x + 3)(x + 7)}{(x + 3)} = x + 7
			\end{dmath}

			\begin{dmath}
				\frac{x^2 + 9x + 20}{(x + 4)} = \frac{(x + 4)(x + 5)}{(x + 4)} = x + 5
			\end{dmath}

			\begin{dmath}
				\frac{x^2 + x - 12}{(x - 3)} = \frac{(x - 3)(x + 4)}{(x - 3)} = x + 4
			\end{dmath}

			\begin{dmath}
				\frac{x^2 + x - 20}{x^2 + 2x - 15} = \frac{(x - 4)(x + 5)}{(x - 3)(x + 5)} = \frac{x - 4}{x - 3}
			\end{dmath}

			\begin{dmath}
				\frac{x^2 + 3x + 2}{x^2 + 5x + 4} = \frac{(x + 1)(x + 2)}{(x + 1)(x + 4)} = \frac{x + 2}{x + 4}
			\end{dmath}

			\begin{dmath}
				\frac{x^2 + x - 12}{x^2 - 9x + 18} = \frac{(x - 3)(x + 4)}{(x - 3)(x - 6)} = \frac{x + 4}{x - 6}
			\end{dmath}

			\begin{dmath}
				\frac{2x^2 + 7x + 6}{(x - 5)(x + 2)} = \frac{(2x + 3)(x + 2)}{(x - 5)(x + 2)} = \frac{2x + 3}{x - 5}
			\end{dmath}

			\begin{dmath}
				\frac{2x^2 + 9x - 18}{(x + 6)(x + 1)} = \frac{(2x - 3)(x + 6)}{(x + 6)(x + 1)} = \frac{2x - 3}{x + 1}
			\end{dmath}

			\begin{dmath}
				\frac{3x^2 - 7x + 2}{(3x - 1)(x + 2)} = \frac{(3x - 1)(x - 2)}{(3x - 1)(x + 2)} = \frac{x - 2}{x + 2}
			\end{dmath}

			\begin{dmath}
				\frac{2x^2 + 3x + 1}{x^2 - x - 2} = \frac{(2x + 1)(x + 1)}{(x - 2)(x + 1)} = \frac{2x + 1}{x - 2}
			\end{dmath}

			\begin{dmath}
				\frac{x^2 + 6x + 8}{3x^2 + 7x + 2} = \frac{(x + 4)(x + 2)}{(3x + 1)(x + 2)} = \frac{x + 4}{3x + 1}
			\end{dmath}

			\begin{dmath}
				\frac{2x^2 - 5x - 3}{2x^2 - 9x + 9} = \frac{(2x + 1)(x - 3)}{(2x - 3)(x - 3)} = \frac{2x + 1}{2x - 3}
			\end{dmath}
		\end{subequations}

		\section*{Question 3}
		\text{Find $a$, $b$, and $c$:}
		
		\begin{dmath}
			\frac{6x^3 + 3x^2 - 84x}{6x^2 - 33x + 42} = \frac{ax(x + b)}{x + c}
		\end{dmath}

		\begin{dmath*}
			\frac{6x^3 + 3x^2 - 84x}{6x^2 - 33x + 42} = \frac{3x(2x^2 + x - 28)}{3(2x^2 - 11x + 14)} = \frac{x(2x - 7)(x + 4)}{(2x - 7)(x - 2)} = \frac{x(x + 4)}{x - 2}
		\end{dmath*}

		$\therefore a = 1, b = 4, c = -2$
	\end{center}
\end{document}
